deps/poulet4/lib/P4automata/Examples.v
@@ -168,6 +168,7 @@ Module BabyIP1.
   Inductive header :=
   | HdrIP
   | HdrUDPTCP.
+
   Scheme Equality for header.
   Global Instance header_eqdec: EquivDec.EqDec header eq := header_eq_dec.
   Global Program Instance header_finite: @Finite header _ header_eq_dec :=
@@ -190,9 +191,9 @@ Module BabyIP1.
     match s with
     | Start =>
       {| st_op := OpExtract 20 (HRVar HdrIP);
-         st_trans := P4A.TSel (ESlice (EHdr (HRVar HdrIP)) 20 16)
+         st_trans := P4A.TSel (ESlice (EHdr (HRVar HdrIP)) 19 16)
                               [{| sc_val := VBits [false; false; false; true];
-                                 sc_st := inl ParseUDP |};
+                                  sc_st := inl ParseUDP |};
                               {| sc_val := VBits [false; false; false; false];
                                  sc_st := inl ParseTCP |}]
                               (inr false) |}
@@ -204,10 +205,84 @@ Module BabyIP1.
          st_trans := P4A.TGoto _ (inr true) |}
     end.
 
+  Program Definition aut: Syntax.t state header :=
+    {| t_states := states |}.
+  Next Obligation.
+    destruct s; cbv; Lia.lia.
+  Qed.
+
 End BabyIP1.
 
 Module BabyIP2.
+  Inductive state :=
+  | Start
+  | ParseSeq.
+  Scheme Equality for state.
+  Global Instance state_eqdec: EquivDec.EqDec state eq := state_eq_dec.
+  Global Program Instance state_finite: @Finite state _ state_eq_dec :=
+    {| enum := [Start; ParseSeq] |}.
+  Next Obligation.
+    repeat constructor;
+      repeat match goal with
+             | H: List.In _ [] |- _ => apply List.in_nil in H; exfalso; exact H
+             | |- ~ List.In _ [] => apply List.in_nil
+             | |- ~ List.In _ (_ :: _) => unfold not; intros
+             | H: List.In _ (_::_) |- _ => inversion H; clear H
+             | _ => discriminate
+             end.
+  Qed.
+  Next Obligation.
+    destruct x; intuition congruence.
+  Qed.
+
+  Inductive header :=
+  | HdrCombi
+  | HdrSeq.
+
+  Scheme Equality for header.
+  Global Instance header_eqdec: EquivDec.EqDec header eq := header_eq_dec.
+  Global Program Instance header_finite: @Finite header _ header_eq_dec :=
+    {| enum := [HdrCombi; HdrSeq] |}.
+  Next Obligation.
+    repeat constructor;
+      repeat match goal with
+             | H: List.In _ [] |- _ => apply List.in_nil in H; exfalso; exact H
+             | |- ~ List.In _ [] => apply List.in_nil
+             | |- ~ List.In _ (_ :: _) => unfold not; intros
+             | H: List.In _ (_::_) |- _ => inversion H; clear H
+             | _ => discriminate
+             end.
+  Qed.
+  Next Obligation.
+    destruct x; intuition congruence.
+  Qed.
+
+  Definition states (s: state) :=
+    match s with
+    | Start =>
+      {| st_op := OpExtract 40 (HRVar HdrCombi);
+         st_trans := P4A.TSel (ESlice (EHdr (HRVar HdrCombi)) 19 16)
+                              [{| sc_val := VBits [false; false; false; true];
+                                  sc_st := inr true |};
+                              {| sc_val := VBits [false; false; false; false];
+                                 sc_st := inl ParseSeq |}]
+                              (inr false) |}
+    | ParseSeq =>
+      {| st_op := OpExtract 8 (HRVar HdrSeq);
+         st_trans := P4A.TGoto _ (inr true) |}
+    end.
+
+  Program Definition aut: Syntax.t state header :=
+    {| t_states := states |}.
+  Next Obligation.
+    destruct s; cbv; Lia.lia.
+  Qed.
+
 End BabyIP2.
+
+Module BabyIP.
+  Definition aut := Sum.sum BabyIP1.aut BabyIP2.aut.
+End BabyIP.
 
 Module MPLS1.
 End MPLS1.
